Implement filtering for multiples

main.dfy
@@ -1,3 +1,89 @@
+predicate Contains(xs: array<int>, x: int)
+reads xs
+{
+    exists i :: 0 <= i < xs.Length && xs[i] == x
+}
+
+// Removes the i-th element of an array.
+method RemoveIth(xs: array<int>, i: int) returns (ys: array<int>)
+requires xs.Length >= 1
+requires 0 <= i < xs.Length
+ensures ys.Length == xs.Length - 1
+ensures forall k :: 0 <= k < i ==> xs[k] == ys[k]
+ensures forall k :: i + 1 <= k < xs.Length ==> xs[k] == ys[k - 1]
+ensures forall k :: (0 <= k < xs.Length && k != i) ==> Contains(ys, xs[k])
+{
+    ys := new int[xs.Length - 1];
+    // Copying first part of xs into ys
+    var j := 0;
+    while(j < i)
+    invariant forall k :: 0 <= k < j ==> k < ys.Length && ys[k] == xs[k]
+    {
+        ys[j] := xs[j];
+        j := j + 1;
+    }
+    // Copying second part of xs into ys
+    j := i + 1;
+    while(j < xs.Length)
+    invariant forall k :: 0 <= k < i ==> ys[k] == xs[k]
+    invariant forall k :: i + 1 <= k < j ==> k - 1 < ys.Length && ys[k - 1] == xs[k]
+    {
+        ys[j - 1] := xs[j];
+        j := j + 1;
+    }
+}
+
+// Appends an integer x to the end of an array xs.
+method Append(xs: array<int>, x: int) returns (ys: array<int>)
+ensures ys.Length == xs.Length + 1
+ensures forall j :: 0 <= j < xs.Length ==> xs[j] == ys[j]
+ensures ys[xs.Length] == x
+{
+    ys := new int[xs.Length + 1];
+    var j := 0;
+    while(j < xs.Length)
+    invariant forall k :: 0 <= k < j ==> k < xs.Length && ys[k] == xs[k]
+    {
+        ys[j] := xs[j];
+        j := j + 1;
+    }
+    ys[xs.Length] := x;
+}
+
+// Filters away all multiples of m from an array xs
+method RemoveMultiples(xs: array<int>, m: int) returns (sieved: array<int>)
+requires m > 0
+ensures forall k :: 0 <= k < sieved.Length ==> sieved[k] % m != 0
+ensures forall k :: 0 <= k < xs.Length ==> xs[k] % m != 0 ==> Contains(sieved, xs[k])
+ensures sieved.Length <= xs.Length
+{
+    sieved := new int[0];
+    var i := 0;
+    while(i < xs.Length)
+    decreases xs.Length - i
+    invariant i <= xs.Length
+    invariant forall k :: 0 <= k < sieved.Length ==> sieved[k] % m != 0
+    invariant forall k :: 0 <= k < i ==> k < xs.Length && xs[k] % m != 0 ==> Contains(sieved, xs[k])
+    invariant sieved.Length <= i
+    {
+        if(xs[i] % m != 0) {
+            sieved := Append(sieved, xs[i]);
+        }
+        i := i + 1;
+    }
+}
+
+method PrintArr(xs: array<int>) {
+    var i := 0;
+    while(i < xs.Length) {
+        print xs[i];
+        print "\n";
+        i := i + 1;
+    }
+}
+
 method Main() {
-    print "hello world";
+    var xs := new int[][11, 22, 33, 44, 55, 66, 77];
+    var ys := RemoveMultiples(xs, 3);
+    PrintArr(ys);
 }
